@prefix : <https://schema.org/> .
@prefix dc: <http://purl.org/dc/terms/> .
@prefix owl: <http://www.w3.org/2002/07/owl#> .
@prefix rdf: <http://www.w3.org/1999/02/22-rdf-syntax-ns#> .
@prefix rdfs: <http://www.w3.org/2000/01/rdf-schema#> .
@prefix xml: <http://www.w3.org/XML/1998/namespace> .
@prefix xsd: <http://www.w3.org/2001/XMLSchema#> .

:ExternalEnumeration a rdfs:Class;
    rdfs:label "ExternalEnumeration";
    rdfs:subClassOf :Enumeration;
    rdfs:comment "Base type for external enumerations" .

:externalUriPrefix a rdf:Property ;
    rdfs:label "externalUriPrefix" ;
    :domainIncludes :ExternalEnumeration ;
    :rangeIncludes :URL ;
    rdfs:comment "URI Prefix for extern Enumeration member terms." .

:externalUriExample a rdf:Property ;
    rdfs:label "externalUriExample" ;
    :domainIncludes :ExternalEnumeration ;
    :rangeIncludes :URL ;
    rdfs:comment "Example URI for an external enumeration member." .

:externalUriSource a rdf:Property ;
    rdfs:label "externalUriSource" ;
    :domainIncludes :ExternalEnumeration ;
    :rangeIncludes :URL ;
    rdfs:comment "Link to externally provided source information for external enumeration." .

:LCNAF a :ExternalEnumeration;
    rdfs:label "LCNAF";
    rdfs:comment "**Library of Congress Name Authority File** - External enumeration values for agents, such as person and organization, names curated by The Library of Congress.";
    :externalUriPrefix "http://id.loc.gov/authorities/names/";
    :externalUriExample "http://id.loc.gov/authorities/names/no2017146789";
    :externalUriSource "https://id.loc.gov/authorities/names.html".

:FoodOn a :ExternalEnumeration;
    rdfs:label "FoodOn";
    rdfs:comment "**FoodOn Food Ontology** - External enumeration values for foods. For example [Butter](http://purl.obolibrary.org/obo/FOODON_03310351), [Burrito](http://purl.obolibrary.org/obo/FOODON_00002510), [Cannelloni](http://purl.obolibrary.org/obo/FOODON_00002831).";
    :externalUriPrefix "http://purl.obolibrary.org/obo/";
    :externalUriExample "http://purl.obolibrary.org/obo/FOODON_03310351";
    :externalUriExample "http://purl.obolibrary.org/obo/FOODON_00002510";
    :externalUriExample "http://purl.obolibrary.org/obo/FOODON_00002831";
    :externalUriSource "https://foodon.org/".

